dictionaries.

Lists.v
@@ -680,3 +680,48 @@ Proof.
   simpl. reflexivity.
   simpl. reflexivity.
 Qed.
+
+(* Dictionaries *)
+
+Module Dictionary.
+
+Inductive dictionary : Type :=
+  | empty : dictionary
+  | record : nat -> nat -> dictionary -> dictionary.
+
+Definition insert (key value : nat) (d : dictionary) : dictionary :=
+  (record key value d).
+
+Fixpoint find (key : nat) (d : dictionary) : natoption :=
+  match d with
+  | empty => None
+  | record k v d' => if (beq_nat key k)
+                       then (Some v)
+                       else (find key d')
+  end.
+
+(* Exercise: 1 star (dictionary_invariant1) *)
+
+Theorem dictionary_invariant1' : forall(d : dictionary) (k v: nat),
+  (find k (insert k v d)) = Some v.
+Proof.
+  simpl.
+  intros d k.
+  rewrite <- beq_nat_refl.
+  reflexivity.
+Qed.
+
+(* Exercise: 1 star (dictionary_invariant2) *)
+
+Theorem dictionary_invariant2' : forall(d : dictionary) (m n o: nat),
+  beq_nat m n = false -> find m d = find m (insert n o d).
+Proof.
+  intros d m n o h.
+  simpl.
+  rewrite -> h.
+  reflexivity.
+Qed.
+
+End Dictionary.
+
+End NatList.
